brainfuck_semantics.thy
@@ -1,0 +1,121 @@
+(*formal semantics of brainfuck*)
+
+theory brainfuck_semantics
+imports Main
+  "~~/src/HOL/Word/Word"
+begin
+
+type_synonym byte = "8 word"
+lemma "(256 :: byte) = 0" by simp
+
+
+datatype bf_cmd = BF_RIGHT  --">, increment the data pointer (to point to the next cell to the right)." 
+                | BF_LEFT  --"<, decrement the data pointer (to point to the next cell to the left)."
+                | BF_PLUS  --"+, increment the byte at the data pointer."
+                | BF_MINUS  --"-, decrement the byte at the data pointer."
+                | BF_OUTPUT  --"., output the byte at the data pointer."
+                | BF_INPUT  --",, accept one byte of input, storing its value in the byte at the data pointer."
+                | BF_LOOPSTART   --"[, while data pointer is not zero"
+                | BF_LOOPEND --"]"
+
+
+datatype tape = Tape "byte list" byte    "byte list"
+--"                   left       current right"
+--" left is ordered in reverse"
+--"tape is (rev left)@[current]@right"
+
+
+datatype outp = Outp "byte list"
+datatype inp = Inp "byte list"
+datatype state = Error | Normal tape inp outp
+
+(*not sure if this syntax annotation awakens daemons*)
+datatype tape_visual = B byte ("_\<^sub>b\<^isub>y\<^isub>t\<^isub>e")| XR ("\<longrightarrow>\<^isub>p\<^isub>c")| XL ("\<longleftarrow>\<^isub>p\<^isub>c")
+
+fun print_state :: "state \<Rightarrow> (tape_visual list \<times> byte list \<times> byte list) option" where
+  "print_state Error = None" |
+  "print_state (Normal (Tape lt c rt) (Inp inp) (Outp outp)) = Some ((map B (rev lt))@[XR]@[B c]@[XL]@(map B rt), inp, rev outp)"
+
+
+inductive eval_bf :: "bf_cmd list \<Rightarrow> state \<Rightarrow> state \<Rightarrow> bool"  where
+init:  "s = s' \<Longrightarrow> eval_bf [] s s'" |
+       "eval_bf [BF_RIGHT] (Normal (Tape lt c []) inp outp)       (Normal (Tape (c#lt) 0 []) inp outp)" |
+       "eval_bf [BF_RIGHT] (Normal (Tape lt c (rt#rts)) inp outp) (Normal (Tape (c#lt) rt rts) inp outp)" |
+       "eval_bf [BF_LEFT]  (Normal (Tape [] c rt) inp outp)       Error"  |
+       "eval_bf [BF_LEFT]  (Normal (Tape (lt#lts) c rt) inp outp) (Normal (Tape lts lt (c#rt)) inp outp)" |
+       "eval_bf [BF_PLUS]  (Normal (Tape lt c rt) inp outp)       (Normal (Tape lt (c + 1) rt) inp outp)" |
+       "eval_bf [BF_MINUS] (Normal (Tape lt c rt) inp outp)       (Normal (Tape lt (c - 1) rt) inp outp)" |
+       "eval_bf [BF_OUTPUT] (Normal (Tape lt c rt) inp (Outp outp))     (Normal (Tape lt c rt) inp (Outp (c#outp)))" |
+       "eval_bf [BF_INPUT]  (Normal (Tape lt _ rt) (Inp []) outp)       (Normal (Tape lt 0 rt) (Inp []) outp)" |
+       "eval_bf [BF_INPUT]  (Normal (Tape lt _ rt) (Inp (i#is)) outp)   (Normal (Tape lt i rt) (Inp is) outp)" |
+seq:  "eval_bf code s s' \<Longrightarrow> eval_bf code' s' s'' \<Longrightarrow> eval_bf (code@code') s s''" |
+whileTrue:      "c \<noteq> 0 \<Longrightarrow> eval_bf code (Normal (Tape lt c rt) inp outp) (Normal (Tape lt'' c'' rt'') inp'' outp'') \<Longrightarrow>
+                  eval_bf ([BF_LOOPSTART]@code@[BF_LOOPEND])  (Normal (Tape lt'' c'' rt'') inp'' outp') (Normal (Tape lt' c' rt') inp' outp') \<Longrightarrow>
+        eval_bf ([BF_LOOPSTART]@code@[BF_LOOPEND])  (Normal (Tape lt c rt) inp outp)       (Normal (Tape lt' c' rt') inp' outp')" |
+whileFalse:      "c = 0 \<Longrightarrow> 
+        eval_bf ([BF_LOOPSTART]@code@[BF_LOOPEND])  (Normal (Tape lt c rt) inp outp)       (Normal (Tape lt c rt) inp outp)" 
+
+
+inductive_cases b_bf_init: "eval_bf [] s s'"
+thm b_bf_init
+inductive_cases b_bf_while: "eval_bf (BF_LOOPSTART # code @ [BF_LOOPEND]) s s'"
+thm b_bf_while
+
+lemma subst1: "cmd#code' = [cmd]@code'" by (metis append_Cons append_Nil)
+
+lemma seq': "eval_bf [cmd] s s' \<Longrightarrow> eval_bf code' s' s'' \<Longrightarrow> eval_bf (cmd#code') s s''"
+apply(subst subst1)
+apply(rule eval_bf.seq)
+by(auto)
+
+lemma seq_while_split: "eval_bf ([BF_LOOPSTART]@code@[BF_LOOPEND]) s si \<Longrightarrow> eval_bf (code') si s'
+   \<Longrightarrow> eval_bf ([BF_LOOPSTART]@code@[BF_LOOPEND]@code') s s'"
+  apply(simp)
+  apply(rule eval_bf.seq[of "[BF_LOOPSTART]@code@[BF_LOOPEND]" s si "code'", simplified])
+by(auto intro: eval_bf.intros)
+
+
+lemma "eval_bf [] (Normal (Tape [] 0 []) inp outp) (Normal (Tape [] 0 []) inp outp)"
+  by(simp add: eval_bf.intros)
+
+lemma "eval_bf [BF_PLUS, BF_OUTPUT] (Normal (Tape [] 0 []) inp (Outp [])) (Normal (Tape [] 1 []) inp (Outp [1]))"
+  apply(rule seq')
+  apply(auto intro: eval_bf.intros)
+ done
+
+code_pred eval_bf .
+thm eval_bf.equation (*empty??*)
+thm eval_bf_def
+
+definition bf_hello_world :: "bf_cmd list" where
+  "bf_hello_world \<equiv> 
+BF_PLUS#BF_PLUS#BF_PLUS#BF_PLUS#BF_PLUS#BF_PLUS#BF_PLUS#BF_PLUS#BF_PLUS#BF_PLUS#BF_LOOPSTART#BF_RIGHT#BF_PLUS#BF_PLUS#BF_PLUS#BF_PLUS#BF_PLUS#BF_PLUS#BF_PLUS#BF_RIGHT#BF_PLUS#BF_PLUS#BF_PLUS#BF_PLUS#BF_PLUS#BF_PLUS#BF_PLUS#BF_PLUS#BF_PLUS#BF_PLUS#BF_RIGHT#BF_PLUS#BF_PLUS#BF_PLUS#BF_RIGHT#BF_PLUS#BF_LEFT#BF_LEFT#BF_LEFT#BF_LEFT#BF_MINUS#BF_LOOPEND#BF_RIGHT#BF_PLUS#BF_PLUS#BF_OUTPUT#BF_RIGHT#BF_PLUS#BF_OUTPUT#BF_PLUS#BF_PLUS#BF_PLUS#BF_PLUS#BF_PLUS#BF_PLUS#BF_PLUS#BF_OUTPUT#BF_OUTPUT#BF_PLUS#BF_PLUS#BF_PLUS#BF_OUTPUT#BF_RIGHT#BF_PLUS#BF_PLUS#BF_OUTPUT#BF_LEFT#BF_LEFT#BF_PLUS#BF_PLUS#BF_PLUS#BF_PLUS#BF_PLUS#BF_PLUS#BF_PLUS#BF_PLUS#BF_PLUS#BF_PLUS#BF_PLUS#BF_PLUS#BF_PLUS#BF_PLUS#BF_PLUS#BF_OUTPUT#BF_RIGHT#BF_OUTPUT#BF_PLUS#BF_PLUS#BF_PLUS#BF_OUTPUT#BF_MINUS#BF_MINUS#BF_MINUS#BF_MINUS#BF_MINUS#BF_MINUS#BF_OUTPUT#BF_MINUS#BF_MINUS#BF_MINUS#BF_MINUS#BF_MINUS#BF_MINUS#BF_MINUS#BF_MINUS#BF_OUTPUT#BF_RIGHT#BF_PLUS#BF_OUTPUT#BF_RIGHT#[]
+ "
+
+definition hello_world_ascii :: "byte list" where
+  "hello_world_ascii \<equiv> [72, 101, 108, 108, 111, 32, 87, 111, 114, 108, 100, 33]"
+
+(*why u no work??*)
+values "{zs. eval_bf bf_hello_world (Normal (Tape [] 0 []) (Inp []) (Outp [])) zs}"
+
+lemma hello_world: "eval_bf bf_hello_world 
+    (Normal (Tape [] 0 []) (Inp []) (Outp [])) 
+    (Normal (Tape [33, 100, 87, 0] 10 []) (Inp []) (Outp (rev hello_world_ascii)))"
+apply(simp add: hello_world_ascii_def bf_hello_world_def)
+  apply(rule seq')
+  apply(auto intro: eval_bf.intros)
+  apply(rule seq', auto intro: eval_bf.intros)+
+  apply(rule seq_while_split[of "[BF_RIGHT, BF_PLUS, BF_PLUS, BF_PLUS, BF_PLUS, BF_PLUS, BF_PLUS, BF_PLUS, BF_RIGHT, BF_PLUS, BF_PLUS, BF_PLUS,
+             BF_PLUS, BF_PLUS, BF_PLUS, BF_PLUS, BF_PLUS, BF_PLUS, BF_PLUS, BF_RIGHT, BF_PLUS, BF_PLUS, BF_PLUS, BF_RIGHT, BF_PLUS, BF_LEFT,
+             BF_LEFT, BF_LEFT, BF_LEFT, BF_MINUS]", simplified])
+  apply((rule eval_bf.whileTrue[of _ "[BF_RIGHT, BF_PLUS, BF_PLUS, BF_PLUS, BF_PLUS, BF_PLUS, BF_PLUS, BF_PLUS, BF_RIGHT, BF_PLUS, BF_PLUS, BF_PLUS,
+             BF_PLUS, BF_PLUS, BF_PLUS, BF_PLUS, BF_PLUS, BF_PLUS, BF_PLUS, BF_RIGHT, BF_PLUS, BF_PLUS, BF_PLUS, BF_RIGHT, BF_PLUS, BF_LEFT,
+             BF_LEFT, BF_LEFT, BF_LEFT, BF_MINUS]", simplified], simp),
+        (rule seq', auto intro: eval_bf.intros)+)+
+  apply(rule eval_bf.whileFalse[of _ "[BF_RIGHT, BF_PLUS, BF_PLUS, BF_PLUS, BF_PLUS, BF_PLUS, BF_PLUS, BF_PLUS, BF_RIGHT, BF_PLUS, BF_PLUS, BF_PLUS,
+             BF_PLUS, BF_PLUS, BF_PLUS, BF_PLUS, BF_PLUS, BF_PLUS, BF_PLUS, BF_RIGHT, BF_PLUS, BF_PLUS, BF_PLUS, BF_RIGHT, BF_PLUS, BF_LEFT,
+             BF_LEFT, BF_LEFT, BF_LEFT, BF_MINUS]", simplified], simp)
+  apply(rule seq', auto intro: eval_bf.intros)+
+  done
+
+end
